src/tls/Token.UF1CMA.fst
@@ -1,16 +1,21 @@
-(**! Idealizing agile HMAC; independent of TLS, used for TLS 1.3 Finished message payloads and Binders. *)
-module HMAC.UFCMA
+(* Idealizing derived authentication tokens; independent of TLS, used for TLS 1.2 Finished message payloads. *) 
+module Token.UF1CMA
 
+//TODO use this file instead of TLSPRF
 open Mem
 
-open Platform.Bytes
+// this file is adapted from HMAC.UFCMA but simpler, and yield
+// probabilistic security: the advantage of an adversary guessing the
+// random token is just 1/#tokens. (Do we need to enforce a single
+// verification attempt?)
 
-module MM = FStar.Monotonic.Map
+module MR = FStar.Monotonic.RRef
 
 let ipkg = Pkg.ipkg
-
 let model = Flags.model
-let ideal = Flags.ideal_HMAC // secret idealization flag for the UFCMA assumption
+let ideal = Flags.ideal_HMAC 
+// secret idealization flag for the UF1CMA assumption
+//TODO use a separate flag 
 
 type safe (#ip:ipkg) (i:ip.Pkg.t) = b2t ideal /\ ip.Pkg.honest i
 
@@ -23,26 +28,25 @@ private let is_safe (#ip:ipkg) (i:ip.Pkg.t{ip.Pkg.registered i}): ST bool
 
 #set-options "--initial_fuel 1 --max_fuel 1 --initial_ifuel 1 --max_ifuel 1"
 
+// formally agile in the KDF algorithm, which controls the token length. 
 type ha = Hashing.Spec.alg
-type text = bytes
 
 // initial parameters
 noeq type info = {
   parent: r:rgn {~ (is_tls_rgn r)};
   alg: Hashing.Spec.alg; //too loose? Pkg.kdfa;
-  good: text -> bool //TODO: should be Type0 instead of bool, and erased, but hard to propagate
+  good: bool //TODO: should be Type0 instead of bool, and erased, but hard to propagate
 }
 
-type tag (u:info) = lbytes (Hashing.Spec.tagLen u.alg)
+type tag (u:info) = Platform.Bytes.lbytes (Hashing.Spec.tagLen u.alg)
 
 let keylen (u:info): Pkg.keylen = UInt32.uint_to_t (Hashing.Spec.tagLen u.alg)
 type keyrepr (u:info) = Hashing.Spec.hkey u.alg
 
-let goodish (#ip:ipkg) (i:ip.Pkg.t) (u:info) (msg:text) =
-  _: unit{~(safe i) \/ u.good msg}
+let goodish (#ip:ipkg) (i:ip.Pkg.t) (u:info) = _: unit{~(safe i) \/ u.good}
 
-private type log_t (#ip:ipkg) (i:ip.Pkg.t) (u:info) (r:rgn) =
-  MM.t r (tag u * text) (fun (t,v) -> goodish i u v) (fun _ -> True) // could constrain size
+private type log_t (#ip:ipkg) (i:ip.Pkg.t) (u:info) (r:rgn) = 
+  MR.m_rref r (option (goodish #ip i u)) ssa
 
 // runtime (concrete) type of MAC instances
 noeq abstract type concrete_key =
@@ -59,8 +63,8 @@ noeq (* abstract *) type ir_key (ip:ipkg) (i:ip.Pkg.t) =
   | RealKey: ck:concrete_key -> ir_key ip i
 
 type key (ip:ipkg) (i:ip.Pkg.t{ip.Pkg.registered i}) =
-  (if model then
-    k:ir_key ip i{IdealKey? k <==> safe i}
+  (if model 
+  then k:ir_key ip i{IdealKey? k <==> safe i}
   else concrete_key)
 
 let usage (#ip:ipkg) (#i:ip.Pkg.t{ip.Pkg.registered i}) (k:key ip i): GTot info =
@@ -96,7 +100,7 @@ let footprint (#ip:ipkg) (#i:ip.Pkg.t {ip.Pkg.registered i}) (k:key ip i):
   else Set.empty
 
 val create:
-  ip:ipkg -> ha_of_i: (ip.Pkg.t -> ha) -> good_of_i: (ip.Pkg.t -> text -> bool) ->
+  ip:ipkg -> ha_of_i: (ip.Pkg.t -> ha) -> good_of_i: (ip.Pkg.t -> bool) ->
   i:ip.Pkg.t {ip.Pkg.registered i} ->
   u:info {u.alg = ha_of_i i /\ u.good == good_of_i i} -> ST (k:key ip i)
   (requires fun _ -> model)
@@ -112,13 +116,13 @@ let create ip _ _ i u =
     if is_safe i then
       let region: Mem.subrgn u.parent = new_region u.parent in
       assert(~(is_tls_rgn u.parent));
-      let log: log_t #ip i u region = MM.alloc #_ #_ #_ #_ in
+      let log: log_t #ip i u region = MR.m_alloc region None in
       IdealKey ck region log
     else
       RealKey ck in
   k <: key ip i
 
-let coerceT (ip: ipkg) (ha_of_i: ip.Pkg.t -> ha) (good_of_i: ip.Pkg.t -> text -> bool)
+let coerceT (ip: ipkg) (ha_of_i: ip.Pkg.t -> ha) (good_of_i: ip.Pkg.t -> bool)
   (i: ip.Pkg.t {ip.Pkg.registered i /\ ~(safe i)})
   (u: u:info {u.alg = ha_of_i i /\ u.good == good_of_i i})
   (kv: Pkg.lbytes (keylen u)) : GTot (key ip i)
@@ -129,7 +133,7 @@ let coerceT (ip: ipkg) (ha_of_i: ip.Pkg.t -> ha) (good_of_i: ip.Pkg.t -> text ->
   else ck
 
 val coerce:
-  ip: ipkg -> ha_of_i: (ip.Pkg.t -> ha) -> good_of_i: (ip.Pkg.t -> text -> bool) ->
+  ip: ipkg -> ha_of_i: (ip.Pkg.t -> ha) -> good_of_i: (ip.Pkg.t -> bool) ->
   i: ip.Pkg.t {ip.Pkg.registered i /\ ~(safe i)} ->
   u: (u: info {u.alg = ha_of_i i /\ u.good == good_of_i i}) ->
   kv: Pkg.lbytes (keylen u) -> ST (k:key ip i)
@@ -158,43 +162,41 @@ private let get_key (#ip:ipkg) (#i:ip.Pkg.t{ip.Pkg.registered i}) (k:key ip i)
     | RealKey rk -> rk
   else k
 
-val mac:
+val token:
   #ip:ipkg -> #i:ip.Pkg.t{ip.Pkg.registered i} -> k:key ip i ->
-  p:text {(usage k).good p \/ ~(safe i)} ->
   ST (tag (usage k))
-  (requires fun _ -> True)
+  (requires fun _ -> (usage k).good \/ ~(safe i))
   (ensures fun h0 t h1 -> modifies (footprint k) h0 h1)
   // we may be more precise to prove ideal functional correctness,
-  // e,g,  /\ sel h1 k.log = snoc (sel h0 k.log) (Entry t p)
-let mac #ip #i k p =
-  let MAC u kv = get_key k in
-  let t = HMAC.hmac u.alg kv p in
+let token #ip #i k =
+  let MAC _ t = get_key k in
   if is_safe i then
     (let IdealKey _ _ log = k <: ir_key ip i in
-    if None? (MM.lookup log (t, p)) then MM.extend log (t,p) ());
+    log := Some ());
   t
 
 val verify:
   #ip:ipkg -> #i:ip.Pkg.t {ip.Pkg.registered i} -> k:key ip i ->
-  p:text -> t: tag (usage k) -> ST bool
+  t: tag (usage k) -> ST bool
   (requires fun _ -> True)
   (ensures fun h0 b h1 -> 
     modifies_none h0 h1 /\
-    (b /\ safe i ==> (usage k).good p))
-let verify #ip #i k p t =
-  let MAC u kv = get_key k in
-  let verified = HMAC.hmacVerify u.alg kv p t in
+    (b /\ safe i ==> (usage k).good))
+let verify #ip #i k t =
+  let MAC _ t' = get_key k in 
+  let verified = Platform.Bytes.equalBytes t t' in
   if is_safe i then
     // We use the log to correct any verification errors
     let IdealKey _ _ log = k <: ir_key ip i in
-    let valid = Some? (MM.lookup log (t,p)) in
-    verified && valid
+    match !log with 
+    | Some () -> verified 
+    | None    -> false 
   else
     verified
 
 /// For TLS, we'll use something of the form
 ///
-/// let good text =
+/// let good =
 ///   exists digest.
 ///     hashed ha digest /\
 ///     text = hash ha digest /\
@@ -204,11 +206,11 @@ let verify #ip #i k p t =
 /// - which level of abstraction?
 
 type info1 (ip: ipkg) (ha_of_i: ip.Pkg.t -> ha)
-  (good_of_i: ip.Pkg.t -> text -> bool) (i: ip.Pkg.t)
+  (good_of_i: ip.Pkg.t -> bool) (i: ip.Pkg.t)
   =
   a:info{a.alg = ha_of_i i /\ a.good == good_of_i i}
 
-unfold let localpkg (ip: ipkg) (ha_of_i: i:ip.Pkg.t -> ha) (good_of_i: ip.Pkg.t -> text -> bool)
+unfold let localpkg (ip: ipkg) (ha_of_i: i:ip.Pkg.t -> ha) (good_of_i: ip.Pkg.t -> bool)
   : Pure (Pkg.local_pkg ip)
   (requires True) (ensures fun p -> p.Pkg.key == key ip /\ p.Pkg.info == info1 ip ha_of_i good_of_i)
   =
@@ -244,7 +246,7 @@ open FStar.Tactics
 private type id = nat
 private let ip : ipkg = Pkg.Idx id (fun _ -> True) (fun _ -> True) (fun _ -> true)
 
-private let test (r:rgn {~(is_tls_rgn r)}) (v': bytes) (t': Hashing.Spec.tag Hashing.SHA256)
+private let test (r:rgn {~(is_tls_rgn r)}) (t': Hashing.Spec.tag Hashing.SHA256)
   : ST unit
   (requires fun h0 -> model)
   (ensures fun h0 _ h1 -> True)
@@ -252,7 +254,7 @@ private let test (r:rgn {~(is_tls_rgn r)}) (v': bytes) (t': Hashing.Spec.tag Has
   // testing usability of local packages
   let a = Hashing.SHA256 in
   let ha_of_i (i:ip.Pkg.t) = a in
-  let good_of_i (i:ip.Pkg.t) (v:text) = length v = 0 in // a property worth MACing!
+  let good_of_i (i:ip.Pkg.t) = true in // a property worth MACing!
 
   let p = localpkg ip ha_of_i good_of_i in
   let table = mem_alloc (key ip) in
@@ -279,10 +281,6 @@ private let test (r:rgn {~(is_tls_rgn r)}) (v': bytes) (t': Hashing.Spec.tag Has
   //TODO call memoization_ST instead of memoization? We miss this postcondition.
   assume(q.Pkg.package_invariant h0);
 
-  //TODO superficial but hard to prove...
-  // assume(Monotonic.RRef.m_sel h0 (Pkg.itable table) == MM.empty_map ip.Pkg.t (key ip));
-  // assert(MM.fresh (Pkg.itable table) 0 h0);
-  // assert(q.Pkg.define_table == table);
   assert(mem_fresh q.Pkg.define_table 0 h0);
 
   //17-11-23  causing mysterious squash error
@@ -291,107 +289,10 @@ private let test (r:rgn {~(is_tls_rgn r)}) (v': bytes) (t': Hashing.Spec.tag Has
   let k: key ip 0 = Pkg.Pkg?.create q 0 u in
 
   // testing usability of logical payloads
-  let v = empty_bytes in
-  assert(good_of_i 0 v);
-  let t = mac #ip #0 k v in
+  assert(good_of_i 0);
+  let t = token #ip #0 k in
 
-  let b = verify #ip #0 k v' t' in
-  assert(b /\ b2t ideal ==> length v' = 0);
-  //assert false; // sanity check
+  let b = verify #ip #0 k t in
+  assert(b /\ b2t ideal ==> good_of_i 0);
+  // assert false; // sanity check
   ()
-
-(*
-
-/// ------------ older, TLS-specific implementation
-
-//17-10-21 ADAPT: should depend only on agility parameter.
-
-type id =
-| HMAC_Finished of TLSInfo.finishedId
-| HMAC_Binder of TLSInfo.binderId
-
-let alg (i:id) = match i with
-| HMAC_Finished i -> TLSInfo.finishedId_hash i
-| HMAC_Binder i -> TLSInfo.binderId_hash i
-
-//assume
-val authId: id -> Tot bool
-let authId id = false // TODO: move to Flags
-
-type tag (i:id) = tag (alg i)
-
-
-
-// We keep the tag in case we later want to enforce tag authentication
-abstract type entry (i:id) (good: bytes -> Type) =
-  | Entry: t:tag i -> p:bytes { authId i ==> good p } -> entry i good
-
-
-val region: #i:id -> #good:(bytes -> Type) -> k:key i good -> GTot rid
-val keyval: #i:id -> #good:(bytes -> Type) -> k:key i good -> GTot (keyrepr i)
-
-let region #i #good (k:key i good) = k.region
-let keyval #i #good (k:key i good) = k.kv
-
-#set-options "--initial_fuel 1 --max_fuel 1 --initial_ifuel 1 --max_ifuel 1 --z3rlimit 30"
-// todo: mark it as private
-private let gen0 i good (parent:rgn) kv : ST (key i good)
-  (requires (fun _ -> True))
-  (ensures (fun h0 k h1 ->
-    fresh_subregion (region #i #good k) parent h0 h1 /\
-    modifies Set.empty h0 h1
-  )) =
-  let region = new_region parent in
-  let log = ralloc region Seq.createEmpty in
-  Key #i #good #region kv log
-
-val gen: i:id -> good: (bytes -> Type) -> parent: rgn -> ST(key i good)
-  (requires (fun _ -> True))
-  (ensures (fun h0 k h1 ->
-    modifies Set.empty h0 h1 /\
-    fresh_subregion (region #i #good k) parent h0 h1 ))
-let gen i good parent =
-  gen0 i good parent (CoreCrypto.random (keysize i))
-
-val coerce: i:id -> good: (bytes -> Type) -> parent: rgn -> kv:keyrepr i -> ST(key i good)
-  (requires (fun _ -> ~(authId i)))
-  (ensures (fun h0 k h1 ->
-    modifies Set.empty h0 h1 /\
-    fresh_subregion (region #i #good k) parent h0 h1 ))
-let coerce i good parent kv =
-  gen0 i good parent kv
-
-val leak: #i:id -> #good: (bytes -> Type) -> k:key i good {~(authId i)} -> Tot (kv:keyrepr i { kv = keyval k })
-let leak   #i #good k = k.kv
-
-val mac: #i:id -> #good:(bytes -> Type) -> k:key i good -> p:bytes { authId i ==> good p } -> ST(tag i)
-  (requires (fun _ -> True))
-  (ensures (fun h0 t h1 -> modifies (Set.singleton (region k)) h0 h1
-  //  /\
-  //  sel h1 k.log = snoc (sel h0 k.log) (Entry t p)
-  ))
-
-
-// We log every authenticated texts, with their index and resulting tag
-let mac #i #good k p =
-  let p : p:bytes { authId i ==> good p } = p in
-  let t = HMAC.hmac (alg i) k.kv p in
-  let e : entry i good = Entry t p in
-  recall k.log;
-  k.log := snoc !k.log e;
-  t
-
-abstract val matches: #i:id -> #good:(bytes -> Type) -> p:text -> entry i good -> Tot bool
-let matches #i #good p (Entry _ p') = p = p'
-
-val verify: #i:id -> #good:(bytes -> Type) -> k:key i good -> p:bytes -> t:tag i -> ST bool
-  (requires (fun _ -> True))
-  (ensures (fun h0 b h1 -> modifies Set.empty h0 h1 /\ (b /\ authId i ==> good p)))
-
-// We use the log to correct any verification errors
-let verify #i #good k p t =
-  let x = HMAC.hmacVerify (alg i) k.kv p t in
-  let log = !k.log in
-  x &&
-  ( not(authId i) || Some? (seq_find (matches p) log))
-*)
