src/tls/concrete-flags/Flags.fst
@@ -20,3 +20,4 @@ inline_for_extraction let ideal_Sig = false
 inline_for_extraction let ideal_PMS = false
 inline_for_extraction let ideal_PRF = false
 inline_for_extraction let ideal_AEAD = false
+inline_for_extraction let ideal_HMAC = false
