src/tls/ideal-flags/Flags.fst
@@ -1,12 +1,15 @@
 module Flags
 
 assume val model: bool // scaffolding
-assume val ideal_KEF : bool
-assume val ideal_Nonce : bool
-assume val ideal_Sig : bool
-assume val ideal_PMS : bool
-assume val ideal_PRF : bool
-assume val ideal_AEAD: bool
+
+let t = b:bool {b ==> model} 
+assume val ideal_KEF: t
+assume val ideal_Nonce: t
+assume val ideal_Sig: t
+assume val ideal_PMS: t
+assume val ideal_PRF: t
+assume val ideal_AEAD: t
+assume val ideal_HMAC: t
 
 // debug printing flags, one per module; 
 // the refinement enables us to leak secrets for printing.
